isabelle/CompileAll.thy
@@ -1,0 +1,16 @@
+theory CompileAll
+imports 
+  Chapter05_06 
+  Chapter08_3_Evaluation
+  Chapter09_3_Evaluation
+  Chapter10_3_Evaluation
+  Chapter11_3_Evaluation
+  Chapter15_3_Evaluation
+  Chapter16_5_Abbreviation
+  Chapter17
+  Chapter18_3_Evaluation
+begin
+
+datatype OK = OK
+
+end
